implement UniqueKeyInFlight and HostOwnsUniqueKey definition

messageInvariantPrototypes/toylock/hosts.dfy
@@ -84,10 +84,20 @@ module Host {
   ghost predicate NextReceiveStep(c: Constants, v: Variables, v': Variables, msgOps: MessageOps) {
     && msgOps.send.None?
     && msgOps.recv.Some?
-    && msgOps.recv.value.epoch > v.myEpoch
-    && msgOps.recv.value.dst == c.hostId
-    && !v.hasLock
+    && UniqueKeyInFlight(c, v, 0, msgOps.recv.value)   // the 0 literal is a useless dummy value
     && v' == v.(hasLock := true, myEpoch := msgOps.recv.value.epoch)
+  }
+
+  // Key in-flight definition
+  ghost predicate UniqueKeyInFlight(c: Constants, v: Variables, key: UniqueKey, msg: Message) {
+    && msg.dst == c.hostId
+    && !v.hasLock
+    && v.myEpoch < msg.epoch
+  }
+
+  // Key owned by host definition
+  ghost predicate HostOwnsUniqueKey(c: Constants, v: Variables, key: UniqueKey) {
+    && v.hasLock
   }
 
   ghost predicate Next(c: Constants, v: Variables, v': Variables, msgOps: MessageOps)
